UTP/ITree_Designs.thy
@@ -29,7 +29,7 @@ lemma assert_pre [dpre]: "itree_pre (assert b) = (True)\<^sub>e"
      (metis deadlock_def deadlock_trace_to diverge_not_Vis)
 
 lemma Skip_pre [dpre]: "itree_pre Skip = (True)\<^sub>e"
-  by (auto simp add: itree_pre_def Skip_def)
+  by (auto simp add: itree_pre_def Skip_itree_def)
 
 lemma assigns_pre [dpre]: "itree_pre \<langle>\<sigma>\<rangle>\<^sub>a = (True)\<^sub>e"
   by (auto simp add: itree_pre_def assigns_def)
